share/pulse/examples/dice/cbor/CDDL.Spec.ArrayGroup.fsti
@@ -131,6 +131,17 @@ let array_group3_concat_equiv
   (ensures ((a1 `array_group3_concat` a2) `array_group3_equiv` (a1' `array_group3_concat` a2')))
 = ()
 
+val array_group3_concat_assoc
+  (#b: _)
+  (a1 a2 a3: array_group3 b)
+: Lemma
+  (array_group3_concat a1 (array_group3_concat a2 a3) `array_group3_equiv`
+    array_group3_concat (array_group3_concat a1 a2) a3)
+  [SMTPatOr [
+    [SMTPat (array_group3_concat a1 (array_group3_concat a2 a3))];
+    [SMTPat (array_group3_concat (array_group3_concat a1 a2) a3)]
+  ]]
+
 let array_group3_concat_unique_strong
   #b (a1 a3: array_group3 b)
 : Tot prop
@@ -147,128 +158,18 @@ let array_group3_concat_unique_strong
     a1 (l1 `List.Tot.append` l2) == Some (l1, l2)
   )
 
-let array_group3_concat_unique_strong_prop_intro
-  #b (a1 a3: array_group3 b)
-  (l1 l2: (l: list Cbor.raw_data_item { opt_precedes_list l b }))
-  (l3 rem: list Cbor.raw_data_item)
-: Lemma
-  (requires (
-    array_group3_concat_unique_strong a1 a3 /\
-    (a1 l1 == Some (l1, []) /\ a3 l2 == Some (l3, rem))
-  ))
-  (ensures (
-      array_group3_concat a1 a3 (l1 `List.Tot.append` l2) == Some (l1 `List.Tot.append` l3, rem)
-  ))
-= ()
-
-let array_group3_concat_unique_strong_prop_elim_gen
-  #b (a1 a3: array_group3 b)
-  (l: list Cbor.raw_data_item { opt_precedes_list l b })
-  (l' rem: list Cbor.raw_data_item)
-: Lemma
-  (requires (
-    array_group3_concat_unique_strong a1 a3 /\
-    array_group3_concat a1 a3 l == Some (l', rem)
-  ))
-  (ensures (
-      (exists (l1 l2 l3: list Cbor.raw_data_item) .
-        a1 l == Some (l1, l2) /\
-        a1 l1 == Some (l1, []) /\
-        a3 l2 == Some (l3, rem) /\
-        l' == l1 `List.Tot.append` l3
-  )))
-= ()
-
-let array_group3_concat_unique_strong_prop_elim
-  #b (a1 a3: array_group3 b)
-  (l: list Cbor.raw_data_item { opt_precedes_list l b })
-: Lemma
-  (requires (
-    array_group3_concat_unique_strong a1 a3 /\
-    array_group3_concat a1 a3 l == Some (l, [])
-  ))
-  (ensures (
-      (exists (l1 l2: list Cbor.raw_data_item) .
-        a1 l == Some (l1, l2) /\
-        a1 l1 == Some (l1, []) /\
-        a3 l2 == Some (l2, []))
-  ))
-= array_group3_concat_unique_strong_prop_elim_gen a1 a3 l l [];
-  let Some (l1, l2) = a1 l in
-  let Some (l3, _) = a3 l2 in
-  List.Tot.append_l_nil l3
-
-let array_group3_concat_unique_strong_intro
-  #b (a1 a3: array_group3 b)
-: Lemma
-  (requires (
-    forall (l1 l2: (l: list Cbor.raw_data_item { opt_precedes_list l b })) .
-      Some? (a3 l2) ==> (a1 l1 == Some (l1, []) <==> a1 (l1 `List.Tot.append` l2) == Some (l1, l2))
-  ))
-  (ensures (
-    array_group3_concat_unique_strong a1 a3
-  ))
-= ()
-
-let array_group3_concat_unique_strong_elim1
-  #b (a1 a3: array_group3 b)
-: Lemma
-  (requires (
-    array_group3_concat_unique_strong a1 a3
-  ))
-  (ensures (
-    forall (l1 l2: (l: list Cbor.raw_data_item { opt_precedes_list l b })) .
-      Some? (a3 l2) ==> (a1 l1 == Some (l1, []) ==> a1 (l1 `List.Tot.append` l2) == Some (l1, l2))
-  ))
-= ()
-
-let indefinite_description_ghost3
-  #t1 #t2 #t3
-  (p: t1 -> t2 -> t3 -> prop)
-: Ghost (t1 & t2 & t3)
-    (requires (exists x1 x2 x3 . p x1 x2 x3))
-    (ensures (fun (x1, x2, x3) -> p x1 x2 x3))
-= let x1 = FStar.IndefiniteDescription.indefinite_description_ghost t1 (fun x1 -> exists x2 x3 . p x1 x2 x3) in
-  let x2 = FStar.IndefiniteDescription.indefinite_description_ghost t2 (fun x2 -> exists x3 . p x1 x2 x3) in
-  let x3 = FStar.IndefiniteDescription.indefinite_description_ghost t3 (fun x3 -> p x1 x2 x3) in
-  (x1, x2, x3)
-
-let array_group3_concat_unique_strong_elim2
-  #b (a1 a3: array_group3 b)
-: Lemma
-  (requires (array_group3_concat_unique_strong a1 a3))
-  (ensures (
-    forall (l1 l2: (l: list Cbor.raw_data_item { opt_precedes_list l b })) .
-      Some? (a3 l2) ==> (a1 (l1 `List.Tot.append` l2) == Some (l1, l2) ==> a1 l1 == Some (l1, []))
-  ))
-= let prf
-      (l1 l2: (l: list Cbor.raw_data_item { opt_precedes_list l b }))
-  : Lemma
-    ((Some? (a3 l2) /\ a1 (l1 `List.Tot.append` l2) == Some (l1, l2)) ==> a1 l1 == Some (l1, []))
-  = if FStar.StrongExcludedMiddle.strong_excluded_middle (Some? (a3 l2) /\ a1 (l1 `List.Tot.append` l2) == Some ((l1 <: list _), (l2 <: list _)))
-    then begin
-      let Some (l3, rem) = a3 l2 in
-      let l' = l1 `List.Tot.append` l3 in
-      let l = l1 `List.Tot.append` l2 in
-      array_group3_concat_unique_strong_prop_elim_gen a1 a3 l l' rem
-    end
-  in
-  Classical.forall_intro_2 prf
-
-noextract
-let array_group3_concat_unique_strong'
-  #b (a1 a3: array_group3 b)
-: Tot prop
-=
-    forall (l1 l2: (l: list Cbor.raw_data_item { opt_precedes_list l b })) .
-      Some? (a3 l2) ==> (a1 (l1 `List.Tot.append` l2) == Some (l1, l2) <==> a1 l1 == Some (l1, []))
-
 let array_group3_concat_unique_strong_equiv
-  #b (a1 a3: array_group3 b)
+  #b (a1 a1' a3 a3': array_group3 b)
 : Lemma
-  (array_group3_concat_unique_strong a1 a3 <==> array_group3_concat_unique_strong' a1 a3)
-  [SMTPat (array_group3_concat_unique_strong a1 a3)]
-= Classical.move_requires (array_group3_concat_unique_strong_elim2 a1) a3
+  (requires (
+    array_group3_equiv a1 a1' /\
+    array_group3_equiv a3 a3'
+  ))
+  (ensures (
+    array_group3_concat_unique_strong a1 a3 <==>
+    array_group3_concat_unique_strong a1' a3'
+  ))
+= array_group3_concat_equiv a1 a1' a3 a3'
 
 let array_group3_strong_prefix
   #b (a1: array_group3 b)
@@ -276,44 +177,8 @@ let array_group3_strong_prefix
 = forall (l1 l2: (l: list Cbor.raw_data_item { opt_precedes_list l b })) .
     (a1 l1 == Some (l1, []) <==> a1 (l1 `List.Tot.append` l2) == Some (l1, l2))
 
-let array_group3_strong_prefix_empty
-  (b: option Cbor.raw_data_item)
-: Lemma
-  (array_group3_strong_prefix #b array_group3_empty)
-= ()
-
-let array_group3_strong_prefix_implies_concat_unique_strong
-  #b (a1 a3: array_group3 b)
-: Lemma
-  (array_group3_strong_prefix a1 ==> array_group3_concat_unique_strong a1 a3)
-= ()
-
-let array_group3_concat_unique_strong'_strong_prefix
-  #b (a1 a2: array_group3 b)
-: Lemma
-  (requires (
-    array_group3_concat_unique_strong' a1 a2 /\
-    array_group3_strong_prefix a2
-  ))
-  (ensures (
-    array_group3_strong_prefix (array_group3_concat a1 a2)
-  ))
-= let a = array_group3_concat a1 a2 in
-  let prf
-    (l1 l2: (l: list Cbor.raw_data_item { opt_precedes_list l b }))
-  : Lemma
-    (a l1 == Some (l1, []) ==> a (l1 `List.Tot.append` l2) == Some (l1, l2))
-  = if FStar.StrongExcludedMiddle.strong_excluded_middle (a l1 == Some (l1, []))
-    then begin
-      let Some (l11, l12) = a1 l1 in
-      List.Tot.append_assoc l11 l12 l2
-    end
-    else ()
-  in
-  Classical.forall_intro_2 prf
-
-let array_group3_concat_unique_strong_strong_prefix
-  #b (a1 a2: array_group3 b)
+val array_group3_concat_unique_strong_strong_prefix
+  (#b: _) (a1 a2: array_group3 b)
 : Lemma
   (requires (
     array_group3_concat_unique_strong a1 a2 /\
@@ -322,66 +187,14 @@ let array_group3_concat_unique_strong_strong_prefix
   (ensures (
     array_group3_strong_prefix (array_group3_concat a1 a2)
   ))
-= array_group3_concat_unique_strong'_strong_prefix a1 a2
-
-let array_group3_concat_unique_strong_concat
-  #b (a1 a2 a3: array_group3 b)
-: Lemma
-  (requires (
-    array_group3_concat_unique_strong a1 a2
-  ))
-  (ensures (
-    array_group3_concat_unique_strong a1 (array_group3_concat a2 a3)
-  ))
-= ()
 
 let array_group3_choice #b (a1 a3: array_group3 b) : array_group3 b =
   fun l -> match a1 l with
     | None -> a3 l
     | Some l3 -> Some l3
 
-let array_group3_concat_unique_strong_choice_right #b (a1 a2 a3: array_group3 b) : Lemma
-  (requires (
-    array_group3_concat_unique_strong a1 a2 /\
-    array_group3_concat_unique_strong a1 a3
-  ))
-  (ensures (
-    array_group3_concat_unique_strong a1 (array_group3_choice a2 a3)
-  ))
-= ()
-
 let array_group3_disjoint #b (a1 a2: array_group3 b) : Tot prop
 = (forall (l: list Cbor.raw_data_item { opt_precedes_list l b }) . ~ (Some? (a1 l) /\ Some? (a2 l)))
-
-let array_group3_concat_unique_strong_choice_left #b (a1 a2 a3: array_group3 b) : Lemma
-  (requires (
-    array_group3_concat_unique_strong a1 a3 /\
-    array_group3_concat_unique_strong a2 a3 /\
-    array_group3_disjoint a1 a2
-  ))
-  (ensures (
-    array_group3_concat_unique_strong (array_group3_choice a1 a2) a3
-  ))
-= ()
-
-let array_group3_disjoint_sym #b (a1 a2: array_group3 b) : Lemma
-  (array_group3_disjoint a1 a2 <==> array_group3_disjoint a2 a1)
-= ()
-
-let array_group3_disjoint_choice #b (a1 a2 a3: array_group3 b) : Lemma
-  (requires (
-    array_group3_disjoint a1 a2 /\
-    array_group3_disjoint a1 a3
-  ))
-  (ensures (
-    array_group3_disjoint a1 (array_group3_choice a2 a3)
-  ))
-= ()
-
-let array_group3_disjoint_concat #b (a1 a2 a3: array_group3 b) : Lemma
-  (requires (array_group3_disjoint a1 a2))
-  (ensures (array_group3_disjoint a1 (array_group3_concat a2 a3)))
-= ()
 
 let rec array_group3_zero_or_more' #b (a: array_group3 b) (l: list Cbor.raw_data_item { opt_precedes_list l b }) : Ghost (option (list Cbor.raw_data_item & list Cbor.raw_data_item))
   (requires True)
@@ -402,101 +215,23 @@ let rec array_group3_zero_or_more' #b (a: array_group3 b) (l: list Cbor.raw_data
 
 let array_group3_zero_or_more #b : array_group3 b -> array_group3 b = array_group3_zero_or_more'
 
-let rec array_group3_zero_or_more_some
-  #b
+val array_group3_zero_or_more_some
+  (#b: _)
   (a: array_group3 b)
   (l: list Cbor.raw_data_item { opt_precedes_list l b })
 : Lemma
   (ensures (Some? (array_group3_zero_or_more a l)))
-  (decreases List.Tot.length l)
   [SMTPat (array_group3_zero_or_more a l)]
-= match a l with
-  | None -> ()
-  | Some (l1, l2) ->
-    List.Tot.append_length l1 l2;
-    if Nil? l1
-    then ()
-    else array_group3_zero_or_more_some a l2
 
-let array_group3_concat_unique_strong_concat_zero_or_more_right
-  #b (a1 a2 a3: array_group3 b)
+val array_group3_zero_or_more_equiv (#b: _)
+ (a1 a2: array_group3 b)
 : Lemma
-  (requires (
-    array_group3_concat_unique_strong a1 a2 /\
-    array_group3_concat_unique_strong a1 a3
-  ))
-  (ensures (
-    array_group3_concat_unique_strong a1 (array_group3_concat (array_group3_zero_or_more a2) a3)
-  ))
-= ()
+  (requires array_group3_equiv a1 a2)
+  (ensures array_group3_equiv (array_group3_zero_or_more a1) (array_group3_zero_or_more a2))
+  [SMTPat (array_group3_equiv (array_group3_zero_or_more a1) (array_group3_zero_or_more a2))]
 
-let array_group3_concat_unique_strong_zero_or_more_right
-  #b (a1 a2: array_group3 b)
-: Lemma
-  (ensures (
-    array_group3_concat_unique_strong a1 (array_group3_zero_or_more a2) <==> array_group3_strong_prefix a1
-  ))
-= ()
-
-let array_group3_concat_unique_strong'_zero_or_more_left
-  #b (a1 a2: array_group3 b)
-: Lemma
-  (requires (
-    array_group3_disjoint a1 a2 /\
-    array_group3_concat_unique_strong' a1 a1 /\
-    array_group3_concat_unique_strong' a1 a2
-  ))
-  (ensures (
-    array_group3_concat_unique_strong' (array_group3_zero_or_more a1) a2
-  ))
-= let _ : squash (array_group3_disjoint a1 a2) = () in
-  let rec prf
-    (l1 l2: (l: list Cbor.raw_data_item { opt_precedes_list l b }))
-  : Lemma
-    (ensures (
-      Some? (a2 l2) ==> (array_group3_zero_or_more a1 l1 == Some (l1, []) <==> array_group3_zero_or_more a1 (l1 `List.Tot.append` l2) == Some (l1, l2))
-    ))
-    (decreases (List.Tot.length l1))
-  = if Some? (a2 l2)
-    then begin
-      if FStar.StrongExcludedMiddle.strong_excluded_middle (array_group3_zero_or_more a1 l1 == Some (l1, []))
-      then
-        match a1 l1 with
-        | None -> ()
-        | Some (l1l, l1r) ->
-          if Nil? l1l
-          then ()
-          else begin
-            List.Tot.append_length l1l l1r;
-            List.Tot.append_assoc l1l l1r l2;
-            let Some (l1rl, l1rr) = array_group3_zero_or_more a1 l1r in
-            assert (Nil? l1rr);
-            List.Tot.append_l_nil l1rl;
-            prf l1r l2
-          end
-      else if FStar.StrongExcludedMiddle.strong_excluded_middle (array_group3_zero_or_more a1 (l1 `List.Tot.append` l2) == Some (l1, l2))
-      then begin
-        match a1 (l1 `List.Tot.append` l2) with
-        | None -> ()
-        | Some (l12l, l12r) ->
-          let Some (l12rl, l12rr) = array_group3_zero_or_more a1 l12r in
-          assert (l12rr == l2);
-          List.Tot.append_assoc l12l l12rl l2;
-          List.Tot.append_length l12rl l12rr;
-          List.Tot.append_length l12l l12r;
-          List.Tot.append_length l1 l2;
-          if Nil? l12l
-          then ()
-          else begin
-            prf l12rl l2
-          end
-      end
-    end
-  in
-  Classical.forall_intro_2 prf
-
-let array_group3_concat_unique_strong_zero_or_more_left
-  #b (a1 a2: array_group3 b)
+val array_group3_concat_unique_strong_zero_or_more_left
+  (#b: _) (a1 a2: array_group3 b)
 : Lemma
   (requires (
     array_group3_disjoint a1 a2 /\
@@ -506,7 +241,6 @@ let array_group3_concat_unique_strong_zero_or_more_left
   (ensures (
     array_group3_concat_unique_strong (array_group3_zero_or_more a1) a2
   ))
-= array_group3_concat_unique_strong'_zero_or_more_left a1 a2
 
 let array_group3_concat_unique_weak
   #b (a1 a3: array_group3 b)
@@ -523,6 +257,35 @@ let array_group3_concat_unique_weak
     a1 (l1 `List.Tot.append` l2) == Some (l1, l2)
   )
 
+val array_group3_concat_unique_weak_intro
+  (#b: _) (a1 a3: array_group3 b)
+  (prf1:
+    (l: (l: list Cbor.raw_data_item { opt_precedes_list l b })) ->
+    Lemma
+    (requires array_group3_concat a1 a3 l == Some (l, []))
+    (ensures
+      (exists (l1 l2: list Cbor.raw_data_item) .
+        a1 l == Some (l1, l2) /\
+        a1 l1 == Some (l1, []) /\
+        a3 l2 == Some (l2, [])
+    ))
+//    [SMTPat (array_group3_concat a1 a3 l)]
+  )
+  (prf2:
+    (l1: (l: list Cbor.raw_data_item { opt_precedes_list l b })) ->
+    (l2: (l: list Cbor.raw_data_item { opt_precedes_list l b })) ->
+    Lemma
+    (requires
+        a1 l1 == Some (l1, []) /\ a3 l2 == Some (l2, [])
+    )
+    (ensures       
+      a1 (l1 `List.Tot.append` l2) == Some (l1, l2)
+    )
+//    [SMTPat (a1 (l1 `List.Tot.append` l2))]
+  )
+: Lemma
+  (array_group3_concat_unique_weak a1 a3)
+
 let list_append_l_nil
   (#t: Type)
   (l: list t)
@@ -531,94 +294,8 @@ let list_append_l_nil
   [SMTPat (l `List.Tot.append` [])]
 = List.Tot.append_l_nil l
 
-let array_group3_concat_unique_strong_implies_weak
-  #b (a1 a3: array_group3 b)
-: Lemma
-  (array_group3_concat_unique_strong a1 a3 ==> array_group3_concat_unique_weak a1 a3)
-= ()
-
-#push-options "--z3rlimit 16"
-#restart-solver
-
-let array_group3_concat_unique_weak_concat_zero_or_more_right
-  #b (a1 a2 a3: array_group3 b)
-: Lemma
-  (requires (
-    array_group3_concat_unique_strong a1 a2 /\
-    array_group3_concat_unique_weak a1 a3
-  ))
-  (ensures (
-    array_group3_concat_unique_weak a1 (array_group3_concat (array_group3_zero_or_more a2) a3)
-  ))
-= ()
-
-#pop-options
-
-#push-options "--z3rlimit 32"
-#restart-solver
-
-let array_group3_concat_unique_weak_zero_or_more_left'
-  #b (a1 a2: array_group3 b)
-: Lemma
-  (requires (
-    array_group3_disjoint a1 a2 /\
-    array_group3_concat_unique_strong' a1 a1 /\
-    array_group3_concat_unique_weak a1 a2
-  ))
-  (ensures (
-    array_group3_concat_unique_weak (array_group3_zero_or_more a1) a2
-  ))
-= let a10 = a1 in
-  let a1 = array_group3_zero_or_more a10 in
-  let a3 = a2 in
-  let rec prf2
-    (l1 l2: (l: list Cbor.raw_data_item { opt_precedes_list l b }))
-  : Lemma
-    (ensures ((a1 l1 == Some (l1, []) /\ a3 l2 == Some (l2, [])) ==>
-    a1 (l1 `List.Tot.append` l2) == Some (l1, l2)))
-    (decreases (List.Tot.length l1))
-  = if FStar.StrongExcludedMiddle.strong_excluded_middle (a1 l1 == Some (l1, []) /\ a3 l2 == Some (l2, []))
-    then match a10 l1 with
-    | None -> ()
-    | Some (l1l, l1r) ->
-      if Nil? l1l
-      then ()
-      else begin
-        List.Tot.append_length l1l l1r;
-        List.Tot.append_assoc l1l l1r l2;
-        prf2 l1r l2
-      end
-  in
-  let rec prf1
-    (l: (l: list Cbor.raw_data_item { opt_precedes_list l b }))
-  : Lemma
-    (ensures (array_group3_concat a1 a3 l == Some (l, []) ==> (
-      (exists (l1 l2: list Cbor.raw_data_item) .
-        a1 l == Some (l1, l2) /\
-        a1 l1 == Some (l1, []) /\
-        a3 l2 == Some (l2, [])
-    ))))
-    (decreases (List.Tot.length l))
-  = if FStar.StrongExcludedMiddle.strong_excluded_middle (array_group3_concat a1 a3 l == Some (l, []))
-    then match a10 l with
-    | None -> ()
-    | Some (l1l, l1r) ->
-      if Nil? l1l
-      then ()
-      else begin
-        List.Tot.append_length l1l l1r;
-        prf1 l1r;
-        let Some (l2l, l2r) = a1 l1r in
-        List.Tot.append_assoc l1l l2l l2r
-      end
-  in
-  Classical.forall_intro prf1;
-  Classical.forall_intro_2 prf2
-
-#pop-options
-
-let array_group3_concat_unique_weak_zero_or_more_left
-  #b (a1 a2: array_group3 b)
+val array_group3_concat_unique_weak_zero_or_more_left
+  (#b: _) (a1 a2: array_group3 b)
 : Lemma
   (requires (
     array_group3_disjoint a1 a2 /\
@@ -628,84 +305,9 @@ let array_group3_concat_unique_weak_zero_or_more_left
   (ensures (
     array_group3_concat_unique_weak (array_group3_zero_or_more a1) a2
   ))
-= array_group3_concat_unique_weak_zero_or_more_left' a1 a2
 
-let array_group3_concat_unique_weak_zero_or_more_right
-  #b (a1 a2: array_group3 b)
-: Lemma
-  (requires (
-    array_group3_concat_unique_strong a1 a2
-  ))
-  (ensures (
-    array_group3_concat_unique_weak a1 (array_group3_zero_or_more a2)
-  ))
-= ()
-
-#push-options "--z3rlimit 16"
-#restart-solver
-
-let array_group3_concat_unique_weak_zero_or_more'
-  #b (a1 a2: array_group3 b)
-: Lemma
-  (requires (
-    array_group3_concat_unique_strong' a1 a1 /\
-    array_group3_concat_unique_strong' a1 a2 /\
-    array_group3_disjoint a1 a2
-  ))
-  (ensures (
-    array_group3_concat_unique_weak (array_group3_zero_or_more a1) (array_group3_zero_or_more a2)
-  ))
-= let a10 = a1 in
-  let a1 = array_group3_zero_or_more a10 in
-  let a3 = array_group3_zero_or_more a2 in
-  let rec prf2
-    (l1 l2: (l: list Cbor.raw_data_item { opt_precedes_list l b }))
-  : Lemma
-    (ensures ((a1 l1 == Some (l1, []) /\ a3 l2 == Some (l2, [])) ==>
-    a1 (l1 `List.Tot.append` l2) == Some (l1, l2)))
-    (decreases (List.Tot.length l1))
-  = if FStar.StrongExcludedMiddle.strong_excluded_middle (a1 l1 == Some (l1, []) /\ a3 l2 == Some (l2, []))
-    then match a10 l1 with
-    | None -> ()
-    | Some (l1l, l1r) ->
-      if Nil? l1l
-      then ()
-      else begin
-        List.Tot.append_length l1l l1r;
-        List.Tot.append_assoc l1l l1r l2;
-        prf2 l1r l2
-      end
-  in
-  let rec prf1
-    (l: (l: list Cbor.raw_data_item { opt_precedes_list l b }))
-  : Lemma
-    (ensures (array_group3_concat a1 a3 l == Some (l, []) ==> (
-      (exists (l1 l2: list Cbor.raw_data_item) .
-        a1 l == Some (l1, l2) /\
-        a1 l1 == Some (l1, []) /\
-        a3 l2 == Some (l2, [])
-    ))))
-    (decreases (List.Tot.length l))
-  = if FStar.StrongExcludedMiddle.strong_excluded_middle (array_group3_concat a1 a3 l == Some (l, []))
-    then match a10 l with
-    | None -> ()
-    | Some (l1l, l1r) ->
-      if Nil? l1l
-      then ()
-      else begin
-        List.Tot.append_length l1l l1r;
-        prf1 l1r;
-        let Some (l2l, l2r) = a1 l1r in
-        List.Tot.append_assoc l1l l2l l2r
-      end
-  in
-  Classical.forall_intro prf1;
-  Classical.forall_intro_2 prf2
-
-#pop-options
-
-let array_group3_concat_unique_weak_zero_or_more
-  #b (a1 a2: array_group3 b)
+val array_group3_concat_unique_weak_zero_or_more
+  (#b: _) (a1 a2: array_group3 b)
 : Lemma
   (requires (
     array_group3_concat_unique_strong a1 a1 /\
@@ -715,34 +317,79 @@ let array_group3_concat_unique_weak_zero_or_more
   (ensures (
     array_group3_concat_unique_weak (array_group3_zero_or_more a1) (array_group3_zero_or_more a2)
   ))
-= array_group3_concat_unique_weak_zero_or_more' a1 a2
-
-let array_group3_concat_unique_weak_choice_right #b (a1 a2 a3: array_group3 b) : Lemma
-  (requires (
-    array_group3_concat_unique_weak a1 a2 /\
-    array_group3_concat_unique_weak a1 a3
-  ))
-  (ensures (
-    array_group3_concat_unique_weak a1 (array_group3_choice a2 a3)
-  ))
-= ()
-
-let array_group3_concat_unique_weak_choice_left #b (a1 a2 a3: array_group3 b) : Lemma
-  (requires (
-    array_group3_concat_unique_weak a1 a3 /\
-    array_group3_concat_unique_weak a2 a3 /\
-    array_group3_disjoint a1 a2
-  ))
-  (ensures (
-    array_group3_concat_unique_weak (array_group3_choice a1 a2) a3
-  ))
-= ()
 
 let array_group3_one_or_more #b (a: array_group3 b) : array_group3 b =
   a `array_group3_concat` array_group3_zero_or_more a
 
+let array_group3_one_or_more_equiv #b
+ (a1 a2: array_group3 b)
+: Lemma
+  (requires array_group3_equiv a1 a2)
+  (ensures array_group3_equiv (array_group3_one_or_more a1) (array_group3_one_or_more a2))
+  [SMTPat (array_group3_equiv (array_group3_one_or_more a1) (array_group3_one_or_more a2))]
+= array_group3_zero_or_more_equiv a1 a2
+
 let array_group3_zero_or_one #b (a: array_group3 b) : Tot (array_group3 b) =
   a `array_group3_choice` array_group3_empty
+
+val array_group3_concat_unique_strong_concat_left
+  (#b: _)
+  (g1 g2 g3: array_group3 b)
+: Lemma
+  (requires
+    array_group3_concat_unique_strong g1 (array_group3_concat g2 g3) /\
+    array_group3_concat_unique_strong g2 g3 /\
+    array_group3_concat_unique_weak g1 g2
+  )
+  (ensures
+    array_group3_concat_unique_strong (array_group3_concat g1 g2) g3
+  )
+
+val array_group3_concat_unique_strong_zero_or_one_left
+  (#b: _) (a1 a2: array_group3 b)
+: Lemma
+  (requires (
+    array_group3_disjoint a1 a2 /\
+    array_group3_concat_unique_strong a1 a2
+  ))
+  (ensures (
+    array_group3_concat_unique_strong (array_group3_zero_or_one a1) a2
+  ))
+
+val array_group3_concat_unique_strong_one_or_more_left
+  (#b: _) (a1 a2: array_group3 b)
+: Lemma
+  (requires (
+    array_group3_disjoint a1 a2 /\
+    array_group3_concat_unique_strong a1 a1 /\
+    array_group3_concat_unique_strong a1 a2
+  ))
+  (ensures (
+    array_group3_concat_unique_strong (array_group3_one_or_more a1) a2
+  ))
+
+val array_group3_concat_unique_weak_zero_or_one_left
+  (#b: _) (a1 a2: array_group3 b)
+: Lemma
+  (requires (
+    array_group3_disjoint a1 a2 /\
+    array_group3_concat_unique_weak a1 a2
+  ))
+  (ensures (
+    array_group3_concat_unique_weak (array_group3_zero_or_one a1) a2
+  ))
+
+val array_group3_concat_unique_weak_one_or_more_left
+  (#b: _) (a1 a2: array_group3 b)
+: Lemma
+  (requires (
+    array_group3_disjoint a1 a2 /\
+    array_group3_concat_unique_strong a1 a1 /\
+    array_group3_concat_unique_weak a1 a2
+  ))
+  (ensures (
+    array_group3_concat_unique_weak (array_group3_one_or_more a1) a2
+  ))
 
 let array_group3_item (#b: option Cbor.raw_data_item) (t: bounded_typ_gen b) : array_group3 b = fun l ->
   match l with
@@ -776,6 +423,35 @@ let t_array3_equiv
   (ensures (typ_equiv (t_array3 a1) (t_array3 a2)))
 = ()
 
+let close_array_group
+  (#b: _)
+  (t: array_group3 b)
+: Tot (array_group3 b)
+= fun l ->
+    let res = t l in
+    match res with
+    | Some (_, []) -> res
+    | _ -> None
+
+let maybe_close_array_group
+  (#b: _)
+  (t: array_group3 b)
+  (close: bool)
+: Tot (array_group3 b)
+= if close
+  then close_array_group t
+  else t
+
+let array3_close_array_group
+  (#b: _)
+  (a: array_group3 b)
+: Lemma
+  (typ_equiv
+    (t_array3 a)
+    (t_array3 (close_array_group a))
+  )
+= ()
+
 // Recursive type (needed by COSE Section 5.1 "Recipient")
 
 // Inspiring from Barthe et al., Type-Based Termination with Sized
@@ -793,3 +469,4 @@ let rec t_array3_rec
 =
   Cbor.Array? x &&
   match_array_group3 (phi x (t_array3_rec phi)) (Cbor.Array?.v x)
+
